pulse/src/checker/Pulse.Typing.Metatheory.Base.fst
@@ -22,13 +22,11 @@ module RU = Pulse.RuntimeUtils
 module RT = FStar.Reflection.Typing
 
 let admit_st_comp_typing (g:env) (st:st_comp) 
-  : Dv (st_comp_typing g st)
-  = admit(); 
-    let x = fresh g in
-    STC g st x (admit()) (admit()) (admit())
+  : st_comp_typing g st
+  = admit()
 
 let admit_comp_typing (g:env) (c:comp_st)
-  : Dv (comp_typing_u g c)
+  : comp_typing_u g c
   = match c with
     | C_ST st ->
       CT_ST g st (admit_st_comp_typing g st)
@@ -46,7 +44,7 @@ let st_typing_correctness_ctot (#g:env) (#t:st_term) (#c:comp{C_Tot? c})
 
 let st_typing_correctness (#g:env) (#t:st_term) (#c:comp_st) 
                           (_:st_typing g t c)
-  : Dv (comp_typing_u g c)
+  : comp_typing_u g c
   = admit_comp_typing g c
     
 let add_frame_well_typed (#g:env) (#c:comp_st) (ct:comp_typing_u g c)
@@ -65,9 +63,26 @@ let comp_typing_inversion #g #c ct =
 let st_comp_typing_inversion_cofinite (#g:env) (#st:_) (ct:st_comp_typing g st) = 
   admit(), admit(), (fun _ -> admit())
 
-let st_comp_typing_inversion (#g:env) (#st:_) (ct:st_comp_typing g st) = 
+let stc_ty  (#g:env) (#st:_) (ct:st_comp_typing g st) : universe_of g st.res st.u = 
+ let STC g st x ty pre post = ct in ty
+let stc_pre (#g:env) (#st:_) (ct:st_comp_typing g st) : tot_typing g st.pre tm_slprop = 
+  let STC g st x ty pre post = ct in pre
+let stc_x (#g:env) (#st:_) (ct:st_comp_typing g st) : x:Ghost.erased var{fresh_wrt x g (freevars st.post)} = 
+  let STC g st x ty pre post = ct in Ghost.hide x 
+let stc_post (#g:env) (#st:_) (ct:st_comp_typing g st) 
+  : tot_typing (push_binding g (stc_x ct) ppname_default st.res) 
+               (open_term st.post (stc_x ct)) tm_slprop =
   let STC g st x ty pre post = ct in
-  (| ty, pre, x, post |)
+  post
+let st_comp_typing_inversion (#g:env) (#st:_) (ct:st_comp_typing g st) = 
+   (| stc_ty ct, stc_pre ct, stc_x ct, stc_post ct |)
+
+let st_comp_typing_inversion_with_name (#g:env) (#st:_) (ct:st_comp_typing g st) (x:var{fresh_wrt x g (freevars st.post)})
+: (universe_of g st.res st.u &
+   tot_typing g st.pre tm_slprop &
+   tot_typing (push_binding g x ppname_default st.res) (open_term st.post x) tm_slprop)
+= assume (x == Ghost.reveal <| stc_x ct);
+  (stc_ty ct, stc_pre ct, stc_post ct)
 
 let tm_exists_inversion (#g:env) (#u:universe) (#ty:term) (#p:term) 
                         (_:tot_typing g (tm_exists_sl u (as_binder ty) p) tm_slprop)
@@ -100,15 +115,8 @@ let non_informative_c_weakening (g g':env) (g1:env{ pairwise_disjoint g g1 g' })
 let bind_comp_weakening (g:env) (g':env { disjoint g g' })
   (#x:var) (#c1 #c2 #c3:comp) (d:bind_comp (push_env g g') x c1 c2 c3)
   (g1:env { pairwise_disjoint g g1 g' })
-  : Dv (bind_comp (push_env (push_env g g1) g') x c1 c2 c3)
-        (decreases d) =
-  
-  match d with
-  | Bind_comp _ x c1 c2 _ _ _ ->
-    assume (None? (lookup (push_env g g1) x));
-    let y = fresh (push_env (push_env g g1) g') in
-    assume (~ (y `Set.mem` (freevars (comp_post c2))));
-    Bind_comp _ x c1 c2 (RU.magic ()) y (RU.magic ())
+  : bind_comp (push_env (push_env g g1) g') x c1 c2 c3
+  = admit()
 
 let lift_comp_weakening (g:env) (g':env { disjoint g g'})
   (#c1 #c2:comp) (d:lift_comp (push_env g g') c1 c2)
@@ -194,255 +202,256 @@ let comp_typing_weakening (g:env) (g':env { disjoint g g' })
     CT_STGhost _ inames _ (RU.magic ()) (st_comp_typing_weakening g g' d g1)
 
 #push-options "--split_queries no --z3rlimit_factor 8 --fuel 1 --ifuel 1"
-let rec st_typing_weakening g g' t c d g1
-  : Dv (st_typing (push_env (push_env g g1) g') t c)
-        (decreases d) =
+let st_typing_weakening g g' t c d g1
+  : st_typing (push_env (push_env g g1) g') t c
+  = admit () 
+  //       (decreases d) =
   
-  match d with
-  | T_Abs g x q b u body c b_typing body_typing ->
-    // T_Abs is used only at the top, should not come up
-    assume false;
-    let x = fresh (push_env (push_env g g1) g') in
-    T_Abs g x q b u body c (RU.magic #(tot_typing _ _ _) ()) 
-                          (st_typing_weakening g g' body c body_typing g1)
-  | T_STApp _ head ty q res arg _ _ ->
-    T_STApp _ head ty q res arg (RU.magic #(tot_typing _ _ _) ()) (RU.magic #(tot_typing _ _ _) ())
+  // match d with
+  // | T_Abs g x q b u body c b_typing body_typing ->
+  //   // T_Abs is used only at the top, should not come up
+  //   assume false;
+  //   let x = fresh (push_env (push_env g g1) g') in
+  //   T_Abs g x q b u body c (RU.magic #(tot_typing _ _ _) ()) 
+  //                         (st_typing_weakening g g' body c body_typing g1)
+  // | T_STApp _ head ty q res arg _ _ ->
+  //   T_STApp _ head ty q res arg (RU.magic #(tot_typing _ _ _) ()) (RU.magic #(tot_typing _ _ _) ())
 
-  | T_STGhostApp _ head ty q res arg _ _ _ _ ->
-    // candidate for renaming
-    let x = fresh (push_env (push_env g g1) g') in
-    assume (~ (x `Set.mem` freevars_comp res));
-    T_STGhostApp _ head ty q res arg x (RU.magic ()) (RU.magic ()) (RU.magic ())
+  // | T_STGhostApp _ head ty q res arg _ _ _ _ ->
+  //   // candidate for renaming
+  //   let x = fresh (push_env (push_env g g1) g') in
+  //   assume (~ (x `Set.mem` freevars_comp res));
+  //   T_STGhostApp _ head ty q res arg x (RU.magic ()) (RU.magic ()) (RU.magic ())
 
-  | T_Return _ c use_eq u t e post x_old _ _ _ ->
-    let x = fresh (push_env (push_env g g1) g') in
-    assume (~ (x `Set.mem` freevars post));
-    // x is only used to open and then close
-    assume (comp_return c use_eq u t e post x_old ==
-            comp_return c use_eq u t e post x);
-    T_Return _ c use_eq u t e post x (RU.magic ()) (RU.magic ()) (RU.magic ())
+  // | T_Return _ c use_eq u t e post x_old _ _ _ ->
+  //   let x = fresh (push_env (push_env g g1) g') in
+  //   assume (~ (x `Set.mem` freevars post));
+  //   // x is only used to open and then close
+  //   assume (comp_return c use_eq u t e post x_old ==
+  //           comp_return c use_eq u t e post x);
+  //   T_Return _ c use_eq u t e post x (RU.magic ()) (RU.magic ()) (RU.magic ())
 
-  | T_Lift _ e c1 c2 d_c1 d_lift ->
-    T_Lift _ e c1 c2 (st_typing_weakening g g' e c1 d_c1 g1)
-                     (lift_comp_weakening g g' d_lift g1)
+  // | T_Lift _ e c1 c2 d_c1 d_lift ->
+  //   T_Lift _ e c1 c2 (st_typing_weakening g g' e c1 d_c1 g1)
+  //                    (lift_comp_weakening g g' d_lift g1)
 
-  | T_Bind _ e1 e2 c1 c2 b x c d_e1 _ d_e2 d_bc ->
-    let d_e1 : st_typing (push_env (push_env g g1) g') e1 c1 =
-      st_typing_weakening g g' e1 c1 d_e1 g1 in
-    //
-    // When we call it, g' will actually be empty
-    // And they way bind checker invokes the lemma, we also know x is not in g1
-    // But we must fix it cleanly
-    // Perhaps typing rules should take a thunk, fun (x:var) ...
-    //
-    assume (~ (x `Set.mem` dom g'));
-    assume (~ (x `Set.mem` dom g1));
-    let d_e2
-      : st_typing (push_binding (push_env g g') x ppname_default (comp_res c1))
-                  (open_st_term_nv e2 (b.binder_ppname, x))
-                  c2 = d_e2 in
-    assert (equal (push_binding (push_env g g') x ppname_default (comp_res c1))
-                  (push_env g (push_binding g' x ppname_default (comp_res c1))));
-    let d_e2
-      : st_typing (push_env g (push_binding g' x ppname_default (comp_res c1)))
-                  (open_st_term_nv e2 (b.binder_ppname, x))
-                  c2 = d_e2 in
-    let d_e2
-      : st_typing (push_env (push_env g g1) (push_binding g' x ppname_default (comp_res c1)))
-                  (open_st_term_nv e2 (b.binder_ppname, x))
-                  c2 = st_typing_weakening g (push_binding g' x ppname_default (comp_res c1)) _ _ d_e2 g1 in
-    assert (equal (push_env (push_env g g1) (push_binding g' x ppname_default (comp_res c1)))
-                  (push_binding (push_env (push_env g g1) g') x ppname_default (comp_res c1)));
-    let d_e2
-      : st_typing (push_binding (push_env (push_env g g1) g') x ppname_default (comp_res c1))
-                  (open_st_term_nv e2 (b.binder_ppname, x))
-                  c2 = d_e2 in
-    let d_bc = bind_comp_weakening g g' d_bc g1 in
-    T_Bind _ e1 e2 c1 c2 b x c d_e1 (RU.magic ()) d_e2 d_bc
+  // | T_Bind _ e1 e2 c1 c2 b x c d_e1 _ d_e2 d_bc ->
+  //   let d_e1 : st_typing (push_env (push_env g g1) g') e1 c1 =
+  //     st_typing_weakening g g' e1 c1 d_e1 g1 in
+  //   //
+  //   // When we call it, g' will actually be empty
+  //   // And they way bind checker invokes the lemma, we also know x is not in g1
+  //   // But we must fix it cleanly
+  //   // Perhaps typing rules should take a thunk, fun (x:var) ...
+  //   //
+  //   assume (~ (x `Set.mem` dom g'));
+  //   assume (~ (x `Set.mem` dom g1));
+  //   let d_e2
+  //     : st_typing (push_binding (push_env g g') x ppname_default (comp_res c1))
+  //                 (open_st_term_nv e2 (b.binder_ppname, x))
+  //                 c2 = d_e2 in
+  //   assert (equal (push_binding (push_env g g') x ppname_default (comp_res c1))
+  //                 (push_env g (push_binding g' x ppname_default (comp_res c1))));
+  //   let d_e2
+  //     : st_typing (push_env g (push_binding g' x ppname_default (comp_res c1)))
+  //                 (open_st_term_nv e2 (b.binder_ppname, x))
+  //                 c2 = d_e2 in
+  //   let d_e2
+  //     : st_typing (push_env (push_env g g1) (push_binding g' x ppname_default (comp_res c1)))
+  //                 (open_st_term_nv e2 (b.binder_ppname, x))
+  //                 c2 = st_typing_weakening g (push_binding g' x ppname_default (comp_res c1)) _ _ d_e2 g1 in
+  //   assert (equal (push_env (push_env g g1) (push_binding g' x ppname_default (comp_res c1)))
+  //                 (push_binding (push_env (push_env g g1) g') x ppname_default (comp_res c1)));
+  //   let d_e2
+  //     : st_typing (push_binding (push_env (push_env g g1) g') x ppname_default (comp_res c1))
+  //                 (open_st_term_nv e2 (b.binder_ppname, x))
+  //                 c2 = d_e2 in
+  //   let d_bc = bind_comp_weakening g g' d_bc g1 in
+  //   T_Bind _ e1 e2 c1 c2 b x c d_e1 (RU.magic ()) d_e2 d_bc
 
-  | T_BindFn _ e1 e2 c1 c2 b x d_e1 u _ d_e2 c2_typing  ->
-    let d_e1 : st_typing (push_env (push_env g g1) g') e1 c1 =
-      st_typing_weakening g g' e1 c1 d_e1 g1 in
-    //
-    // When we call it, g' will actually be empty
-    // And they way bind checker invokes the lemma, we also know x is not in g1
-    // But we must fix it cleanly
-    // Perhaps typing rules should take a thunk, fun (x:var) ...
-    //
-    assume (~ (x `Set.mem` dom g'));
-    assume (~ (x `Set.mem` dom g1));
-    let d_e2
-      : st_typing (push_binding (push_env g g') x ppname_default (comp_res c1))
-                  (open_st_term_nv e2 (b.binder_ppname, x))
-                  c2 = d_e2 in
-    assert (equal (push_binding (push_env g g') x ppname_default (comp_res c1))
-                  (push_env g (push_binding g' x ppname_default (comp_res c1))));
-    let d_e2
-      : st_typing (push_env g (push_binding g' x ppname_default (comp_res c1)))
-                  (open_st_term_nv e2 (b.binder_ppname, x))
-                  c2 = d_e2 in
-    let d_e2
-      : st_typing (push_env (push_env g g1) (push_binding g' x ppname_default (comp_res c1)))
-                  (open_st_term_nv e2 (b.binder_ppname, x))
-                  c2 = st_typing_weakening g (push_binding g' x ppname_default (comp_res c1)) _ _ d_e2 g1 in
-    assert (equal (push_env (push_env g g1) (push_binding g' x ppname_default (comp_res c1)))
-                  (push_binding (push_env (push_env g g1) g') x ppname_default (comp_res c1)));
-    let d_e2
-      : st_typing (push_binding (push_env (push_env g g1) g') x ppname_default (comp_res c1))
-                  (open_st_term_nv e2 (b.binder_ppname, x))
-                  c2 = d_e2 in
-    let c2_typing = comp_typing_weakening g g' c2_typing g1 in
-    T_BindFn _ e1 e2 c1 c2 b x d_e1 u (RU.magic #(tot_typing _ _ _) ()) d_e2 c2_typing
+  // | T_BindFn _ e1 e2 c1 c2 b x d_e1 u _ d_e2 c2_typing  ->
+  //   let d_e1 : st_typing (push_env (push_env g g1) g') e1 c1 =
+  //     st_typing_weakening g g' e1 c1 d_e1 g1 in
+  //   //
+  //   // When we call it, g' will actually be empty
+  //   // And they way bind checker invokes the lemma, we also know x is not in g1
+  //   // But we must fix it cleanly
+  //   // Perhaps typing rules should take a thunk, fun (x:var) ...
+  //   //
+  //   assume (~ (x `Set.mem` dom g'));
+  //   assume (~ (x `Set.mem` dom g1));
+  //   let d_e2
+  //     : st_typing (push_binding (push_env g g') x ppname_default (comp_res c1))
+  //                 (open_st_term_nv e2 (b.binder_ppname, x))
+  //                 c2 = d_e2 in
+  //   assert (equal (push_binding (push_env g g') x ppname_default (comp_res c1))
+  //                 (push_env g (push_binding g' x ppname_default (comp_res c1))));
+  //   let d_e2
+  //     : st_typing (push_env g (push_binding g' x ppname_default (comp_res c1)))
+  //                 (open_st_term_nv e2 (b.binder_ppname, x))
+  //                 c2 = d_e2 in
+  //   let d_e2
+  //     : st_typing (push_env (push_env g g1) (push_binding g' x ppname_default (comp_res c1)))
+  //                 (open_st_term_nv e2 (b.binder_ppname, x))
+  //                 c2 = st_typing_weakening g (push_binding g' x ppname_default (comp_res c1)) _ _ d_e2 g1 in
+  //   assert (equal (push_env (push_env g g1) (push_binding g' x ppname_default (comp_res c1)))
+  //                 (push_binding (push_env (push_env g g1) g') x ppname_default (comp_res c1)));
+  //   let d_e2
+  //     : st_typing (push_binding (push_env (push_env g g1) g') x ppname_default (comp_res c1))
+  //                 (open_st_term_nv e2 (b.binder_ppname, x))
+  //                 c2 = d_e2 in
+  //   let c2_typing = comp_typing_weakening g g' c2_typing g1 in
+  //   T_BindFn _ e1 e2 c1 c2 b x d_e1 u (RU.magic #(tot_typing _ _ _) ()) d_e2 c2_typing
 
-  | T_If _ b e1 e2 c hyp _ d_e1 d_e2 _ ->
-    assume (~ (hyp `Set.mem` dom g'));
-    assume (~ (hyp `Set.mem` dom g1));
-    let d_e1
-      : st_typing (push_binding (push_env g g') hyp ppname_default (mk_eq2 u0 tm_bool b tm_true))
-        e1 c = d_e1 in
-    assert (equal (push_binding (push_env g g') hyp ppname_default (mk_eq2 u0 tm_bool b tm_true))
-                  (push_env g (push_binding g' hyp ppname_default (mk_eq2 u0 tm_bool b tm_true))));
-    let d_e1
-      : st_typing (push_env g (push_binding g' hyp ppname_default (mk_eq2 u0 tm_bool b tm_true)))
-                  e1 c = d_e1 in
-    let d_e1
-      : st_typing (push_env (push_env g g1) (push_binding g' hyp ppname_default (mk_eq2 u0 tm_bool b tm_true)))
-                  e1 c = st_typing_weakening g (push_binding g' hyp ppname_default (mk_eq2 u0 tm_bool b tm_true)) _ _ d_e1 g1 in
-    assert (equal (push_env (push_env g g1) (push_binding g' hyp ppname_default (mk_eq2 u0 tm_bool b tm_true)))
-                  (push_binding (push_env (push_env g g1) g') hyp ppname_default (mk_eq2 u0 tm_bool b tm_true))); 
-    let d_e1
-      : st_typing (push_binding (push_env (push_env g g1) g') hyp ppname_default (mk_eq2 u0 tm_bool b tm_true))
-                  e1 c = d_e1 in
-    let d_e2
-      : st_typing (push_binding (push_env g g') hyp ppname_default (mk_eq2 u0 tm_bool b tm_false))
-                  e2 c = d_e2 in
-    assert (equal (push_binding (push_env g g') hyp ppname_default (mk_eq2 u0 tm_bool b tm_false))
-                  (push_env g (push_binding g' hyp ppname_default (mk_eq2 u0 tm_bool b tm_false))));
-    let d_e2
-      : st_typing (push_env g (push_binding g' hyp ppname_default (mk_eq2 u0 tm_bool b tm_false)))
-                  e2 c = d_e2 in
-    let d_e2
-      : st_typing (push_env (push_env g g1) (push_binding g' hyp ppname_default (mk_eq2 u0 tm_bool b tm_false)))
-                  e2 c = st_typing_weakening g (push_binding g' hyp ppname_default (mk_eq2 u0 tm_bool b tm_false)) _ _ d_e2 g1 in
-    assert (equal (push_env (push_env g g1) (push_binding g' hyp ppname_default (mk_eq2 u0 tm_bool b tm_false)))
-                  (push_binding (push_env (push_env g g1) g') hyp ppname_default (mk_eq2 u0 tm_bool b tm_false))); 
-    let d_e2
-      : st_typing (push_binding (push_env (push_env g g1) g') hyp ppname_default (mk_eq2 u0 tm_bool b tm_false))
-                  e2 c = d_e2 in
+  // | T_If _ b e1 e2 c hyp _ d_e1 d_e2 _ ->
+  //   assume (~ (hyp `Set.mem` dom g'));
+  //   assume (~ (hyp `Set.mem` dom g1));
+  //   let d_e1
+  //     : st_typing (push_binding (push_env g g') hyp ppname_default (mk_eq2 u0 tm_bool b tm_true))
+  //       e1 c = d_e1 in
+  //   assert (equal (push_binding (push_env g g') hyp ppname_default (mk_eq2 u0 tm_bool b tm_true))
+  //                 (push_env g (push_binding g' hyp ppname_default (mk_eq2 u0 tm_bool b tm_true))));
+  //   let d_e1
+  //     : st_typing (push_env g (push_binding g' hyp ppname_default (mk_eq2 u0 tm_bool b tm_true)))
+  //                 e1 c = d_e1 in
+  //   let d_e1
+  //     : st_typing (push_env (push_env g g1) (push_binding g' hyp ppname_default (mk_eq2 u0 tm_bool b tm_true)))
+  //                 e1 c = st_typing_weakening g (push_binding g' hyp ppname_default (mk_eq2 u0 tm_bool b tm_true)) _ _ d_e1 g1 in
+  //   assert (equal (push_env (push_env g g1) (push_binding g' hyp ppname_default (mk_eq2 u0 tm_bool b tm_true)))
+  //                 (push_binding (push_env (push_env g g1) g') hyp ppname_default (mk_eq2 u0 tm_bool b tm_true))); 
+  //   let d_e1
+  //     : st_typing (push_binding (push_env (push_env g g1) g') hyp ppname_default (mk_eq2 u0 tm_bool b tm_true))
+  //                 e1 c = d_e1 in
+  //   let d_e2
+  //     : st_typing (push_binding (push_env g g') hyp ppname_default (mk_eq2 u0 tm_bool b tm_false))
+  //                 e2 c = d_e2 in
+  //   assert (equal (push_binding (push_env g g') hyp ppname_default (mk_eq2 u0 tm_bool b tm_false))
+  //                 (push_env g (push_binding g' hyp ppname_default (mk_eq2 u0 tm_bool b tm_false))));
+  //   let d_e2
+  //     : st_typing (push_env g (push_binding g' hyp ppname_default (mk_eq2 u0 tm_bool b tm_false)))
+  //                 e2 c = d_e2 in
+  //   let d_e2
+  //     : st_typing (push_env (push_env g g1) (push_binding g' hyp ppname_default (mk_eq2 u0 tm_bool b tm_false)))
+  //                 e2 c = st_typing_weakening g (push_binding g' hyp ppname_default (mk_eq2 u0 tm_bool b tm_false)) _ _ d_e2 g1 in
+  //   assert (equal (push_env (push_env g g1) (push_binding g' hyp ppname_default (mk_eq2 u0 tm_bool b tm_false)))
+  //                 (push_binding (push_env (push_env g g1) g') hyp ppname_default (mk_eq2 u0 tm_bool b tm_false))); 
+  //   let d_e2
+  //     : st_typing (push_binding (push_env (push_env g g1) g') hyp ppname_default (mk_eq2 u0 tm_bool b tm_false))
+  //                 e2 c = d_e2 in
 
-    T_If _ b e1 e2 c hyp (RU.magic ()) d_e1 d_e2 (RU.magic ())
+  //   T_If _ b e1 e2 c hyp (RU.magic ()) d_e1 d_e2 (RU.magic ())
   
-  | T_Match _ sc_u sc_ty sc d_sc_ty d_sc c c_typing brs d_brs d_pats_complete ->
-    admit();
-    T_Match (push_env (push_env g g1) g')
-            sc_u sc_ty sc
-            (tot_typing_weakening g g' _ _ d_sc_ty g1)
-            (tot_typing_weakening g g' _ _ d_sc g1)
-            c c_typing 
-            brs d_brs
-            d_pats_complete
+  // | T_Match _ sc_u sc_ty sc d_sc_ty d_sc c c_typing brs d_brs d_pats_complete ->
+  //   admit();
+  //   T_Match (push_env (push_env g g1) g')
+  //           sc_u sc_ty sc
+  //           (tot_typing_weakening g g' _ _ d_sc_ty g1)
+  //           (tot_typing_weakening g g' _ _ d_sc g1)
+  //           c c_typing 
+  //           brs d_brs
+  //           d_pats_complete
 
-  | T_Frame _ e c frame _ d_e ->
-    T_Frame _ e c frame (RU.magic ()) (st_typing_weakening g g' e c d_e g1)
+  // | T_Frame _ e c frame _ d_e ->
+  //   T_Frame _ e c frame (RU.magic ()) (st_typing_weakening g g' e c d_e g1)
 
-  | T_Equiv _ e c c' d_e d_eq ->
-    T_Equiv _ e c c' (st_typing_weakening g g' e c d_e g1) (st_equiv_weakening g g' d_eq g1)
+  // | T_Equiv _ e c c' d_e d_eq ->
+  //   T_Equiv _ e c c' (st_typing_weakening g g' e c d_e g1) (st_equiv_weakening g g' d_eq g1)
 
-  | T_Sub _ e c c' d_e d_sub ->
-    T_Sub _ e c c' (st_typing_weakening g g' e c d_e g1) (st_sub_weakening g g' d_sub g1)
+  // | T_Sub _ e c c' d_e d_sub ->
+  //   T_Sub _ e c c' (st_typing_weakening g g' e c d_e g1) (st_sub_weakening g g' d_sub g1)
 
-  | T_IntroPure _ p _ token -> T_IntroPure _ p (RU.magic ()) (prop_validity_token_weakening token _)
+  // | T_IntroPure _ p _ token -> T_IntroPure _ p (RU.magic ()) (prop_validity_token_weakening token _)
 
-  | T_ElimExists _ u t p x _ _ ->
-    assume (~ (x `Set.mem` dom g'));
-    assume (~ (x `Set.mem` dom g1));
-    T_ElimExists _ u t p x (RU.magic ()) (RU.magic ())
+  // | T_ElimExists _ u t p x _ _ ->
+  //   assume (~ (x `Set.mem` dom g'));
+  //   assume (~ (x `Set.mem` dom g1));
+  //   T_ElimExists _ u t p x (RU.magic ()) (RU.magic ())
 
-  | T_IntroExists _ u b p e _ _ _ ->
-    T_IntroExists _ u b p e (RU.magic ()) (RU.magic ()) (RU.magic ())
+  // | T_IntroExists _ u b p e _ _ _ ->
+  //   T_IntroExists _ u b p e (RU.magic ()) (RU.magic ()) (RU.magic ())
 
-  | T_While _ inv cond body _ cond_typing body_typing ->
-    T_While _ inv cond body (RU.magic ())
-      (st_typing_weakening g g' cond (comp_while_cond ppname_default inv) cond_typing g1)
-      (st_typing_weakening g g' body (comp_while_body ppname_default inv) body_typing g1)
+  // | T_While _ inv cond body _ cond_typing body_typing ->
+  //   T_While _ inv cond body (RU.magic ())
+  //     (st_typing_weakening g g' cond (comp_while_cond ppname_default inv) cond_typing g1)
+  //     (st_typing_weakening g g' body (comp_while_body ppname_default inv) body_typing g1)
 
-  | T_Par _ eL cL eR cR x cL_typing cR_typing eL_typing eR_typing ->
-    assume (~ (x `Set.mem` dom g'));
-    assume (~ (x `Set.mem` dom g1));
-    T_Par _ eL cL eR cR x
-      (comp_typing_weakening g g' cL_typing g1)
-      (comp_typing_weakening g g' cR_typing g1)
-      (st_typing_weakening g g' eL cL eL_typing g1)
-      (st_typing_weakening g g' eR cR eR_typing g1)
+  // | T_Par _ eL cL eR cR x cL_typing cR_typing eL_typing eR_typing ->
+  //   assume (~ (x `Set.mem` dom g'));
+  //   assume (~ (x `Set.mem` dom g1));
+  //   T_Par _ eL cL eR cR x
+  //     (comp_typing_weakening g g' cL_typing g1)
+  //     (comp_typing_weakening g g' cR_typing g1)
+  //     (st_typing_weakening g g' eL cL eL_typing g1)
+  //     (st_typing_weakening g g' eR cR eR_typing g1)
 
-  | T_WithLocal _ ppname init body init_t c x _ _ d_c d_body ->
-    assume (~ (x `Set.mem` dom g'));
-    assume (~ (x `Set.mem` dom g1));
-    let d_body
-      : st_typing (push_binding (push_env g g') x ppname_default (mk_ref init_t))
-                  (open_st_term_nv body (v_as_nv x))
-                  (comp_withlocal_body x init_t init c) = d_body in
-    assert (equal (push_binding (push_env g g') x ppname_default (mk_ref init_t))
-                  (push_env g (push_binding g' x ppname_default (mk_ref init_t))));
-    let d_body
-      : st_typing (push_env g (push_binding g' x ppname_default (mk_ref init_t)))
-                  (open_st_term_nv body (v_as_nv x))
-                  (comp_withlocal_body x init_t init c) = d_body in
-    let d_body
-      : st_typing (push_env (push_env g g1) (push_binding g' x ppname_default (mk_ref init_t)))
-                  (open_st_term_nv body (v_as_nv x))
-                  (comp_withlocal_body x init_t init c)
-      = st_typing_weakening g (push_binding g' x ppname_default (mk_ref init_t))  _ _ d_body g1 in
-    assert (equal (push_env (push_env g g1) (push_binding g' x ppname_default (mk_ref init_t)))
-                  (push_binding (push_env (push_env g g1) g') x ppname_default (mk_ref init_t)));
-    let d_body
-      : st_typing (push_binding (push_env (push_env g g1) g') x ppname_default (mk_ref init_t))
-                  (open_st_term_nv body (v_as_nv x))
-                  (comp_withlocal_body x init_t init c) = d_body in
-    T_WithLocal _ ppname init body init_t c x (RU.magic ()) (RU.magic ())
-      (comp_typing_weakening g g' d_c g1)
-      d_body
+  // | T_WithLocal _ ppname init body init_t c x _ _ d_c d_body ->
+  //   assume (~ (x `Set.mem` dom g'));
+  //   assume (~ (x `Set.mem` dom g1));
+  //   let d_body
+  //     : st_typing (push_binding (push_env g g') x ppname_default (mk_ref init_t))
+  //                 (open_st_term_nv body (v_as_nv x))
+  //                 (comp_withlocal_body x init_t init c) = d_body in
+  //   assert (equal (push_binding (push_env g g') x ppname_default (mk_ref init_t))
+  //                 (push_env g (push_binding g' x ppname_default (mk_ref init_t))));
+  //   let d_body
+  //     : st_typing (push_env g (push_binding g' x ppname_default (mk_ref init_t)))
+  //                 (open_st_term_nv body (v_as_nv x))
+  //                 (comp_withlocal_body x init_t init c) = d_body in
+  //   let d_body
+  //     : st_typing (push_env (push_env g g1) (push_binding g' x ppname_default (mk_ref init_t)))
+  //                 (open_st_term_nv body (v_as_nv x))
+  //                 (comp_withlocal_body x init_t init c)
+  //     = st_typing_weakening g (push_binding g' x ppname_default (mk_ref init_t))  _ _ d_body g1 in
+  //   assert (equal (push_env (push_env g g1) (push_binding g' x ppname_default (mk_ref init_t)))
+  //                 (push_binding (push_env (push_env g g1) g') x ppname_default (mk_ref init_t)));
+  //   let d_body
+  //     : st_typing (push_binding (push_env (push_env g g1) g') x ppname_default (mk_ref init_t))
+  //                 (open_st_term_nv body (v_as_nv x))
+  //                 (comp_withlocal_body x init_t init c) = d_body in
+  //   T_WithLocal _ ppname init body init_t c x (RU.magic ()) (RU.magic ())
+  //     (comp_typing_weakening g g' d_c g1)
+  //     d_body
 
-  | T_WithLocalArray _ ppname init len body init_t c x _ _ _ d_c d_body ->
-    assume (~ (x `Set.mem` dom g'));
-    assume (~ (x `Set.mem` dom g1));
-    let d_body
-      : st_typing (push_binding (push_env g g') x ppname_default (mk_array init_t))
-                  (open_st_term_nv body (v_as_nv x))
-                  (comp_withlocal_array_body x init_t init len c) = d_body in
-    assert (equal (push_binding (push_env g g') x ppname_default (mk_array init_t))
-                  (push_env g (push_binding g' x ppname_default (mk_array init_t))));
-    let d_body
-      : st_typing (push_env g (push_binding g' x ppname_default (mk_array init_t)))
-                  (open_st_term_nv body (v_as_nv x))
-                  (comp_withlocal_array_body x init_t init len c) = d_body in
-    let d_body
-      : st_typing (push_env (push_env g g1) (push_binding g' x ppname_default (mk_array init_t)))
-                  (open_st_term_nv body (v_as_nv x))
-                  (comp_withlocal_array_body x init_t init len c)
-      = st_typing_weakening g (push_binding g' x ppname_default (mk_array init_t))  _ _ d_body g1 in
-    assert (equal (push_env (push_env g g1) (push_binding g' x ppname_default (mk_array init_t)))
-                  (push_binding (push_env (push_env g g1) g') x ppname_default (mk_array init_t)));
-    let d_body
-      : st_typing (push_binding (push_env (push_env g g1) g') x ppname_default (mk_array init_t))
-                  (open_st_term_nv body (v_as_nv x))
-                  (comp_withlocal_array_body x init_t init len c) = d_body in
-    T_WithLocalArray _ ppname init len body init_t c x (RU.magic ()) (RU.magic ()) (RU.magic ())
-      (comp_typing_weakening g g' d_c g1)
-      d_body
+  // | T_WithLocalArray _ ppname init len body init_t c x _ _ _ d_c d_body ->
+  //   assume (~ (x `Set.mem` dom g'));
+  //   assume (~ (x `Set.mem` dom g1));
+  //   let d_body
+  //     : st_typing (push_binding (push_env g g') x ppname_default (mk_array init_t))
+  //                 (open_st_term_nv body (v_as_nv x))
+  //                 (comp_withlocal_array_body x init_t init len c) = d_body in
+  //   assert (equal (push_binding (push_env g g') x ppname_default (mk_array init_t))
+  //                 (push_env g (push_binding g' x ppname_default (mk_array init_t))));
+  //   let d_body
+  //     : st_typing (push_env g (push_binding g' x ppname_default (mk_array init_t)))
+  //                 (open_st_term_nv body (v_as_nv x))
+  //                 (comp_withlocal_array_body x init_t init len c) = d_body in
+  //   let d_body
+  //     : st_typing (push_env (push_env g g1) (push_binding g' x ppname_default (mk_array init_t)))
+  //                 (open_st_term_nv body (v_as_nv x))
+  //                 (comp_withlocal_array_body x init_t init len c)
+  //     = st_typing_weakening g (push_binding g' x ppname_default (mk_array init_t))  _ _ d_body g1 in
+  //   assert (equal (push_env (push_env g g1) (push_binding g' x ppname_default (mk_array init_t)))
+  //                 (push_binding (push_env (push_env g g1) g') x ppname_default (mk_array init_t)));
+  //   let d_body
+  //     : st_typing (push_binding (push_env (push_env g g1) g') x ppname_default (mk_array init_t))
+  //                 (open_st_term_nv body (v_as_nv x))
+  //                 (comp_withlocal_array_body x init_t init len c) = d_body in
+  //   T_WithLocalArray _ ppname init len body init_t c x (RU.magic ()) (RU.magic ()) (RU.magic ())
+  //     (comp_typing_weakening g g' d_c g1)
+  //     d_body
 
-  | T_Rewrite _ p q _ _ -> T_Rewrite _ p q (RU.magic ()) (RU.magic ())
+  // | T_Rewrite _ p q _ _ -> T_Rewrite _ p q (RU.magic ()) (RU.magic ())
 
-  | T_Admit _ c d_c -> T_Admit _ c (comp_typing_weakening g g' d_c g1)
+  // | T_Admit _ c d_c -> T_Admit _ c (comp_typing_weakening g g' d_c g1)
 
-  | T_Unreachable _ c d_c tok ->
-    T_Unreachable _ c (comp_typing_weakening g g' d_c g1) (RU.magic ())  // weaken tok
+  // | T_Unreachable _ c d_c tok ->
+  //   T_Unreachable _ c (comp_typing_weakening g g' d_c g1) (RU.magic ())  // weaken tok
 
-  | T_WithInv  _ _ _ _ _ i_typing p_typing body_typing tok ->
-    T_WithInv _ _ _ _ _ (tot_typing_weakening g g' _ _ i_typing g1)
-                        (tot_typing_weakening g g' _ _ p_typing g1)
-                        (st_typing_weakening g g' _ _ body_typing g1)
-                        (prop_validity_token_weakening tok _)
+  // | T_WithInv  _ _ _ _ _ i_typing p_typing body_typing tok ->
+  //   T_WithInv _ _ _ _ _ (tot_typing_weakening g g' _ _ i_typing g1)
+  //                       (tot_typing_weakening g g' _ _ p_typing g1)
+  //                       (st_typing_weakening g g' _ _ body_typing g1)
+  //                       (prop_validity_token_weakening tok _)
 #pop-options
 
 let non_informative_t_subst (g:env) (x:var) (t:typ) (g':env { pairwise_disjoint g (singleton_env (fstar_env g) x t) g' })
