pulse/src/checker/Pulse.Typing.Printer.fst
@@ -19,79 +19,80 @@ module T = FStar.Tactics
 open Pulse.Syntax.Printer
 open Pulse.Typing
 
-let rec print_st_typing #g #t #c (d:st_typing g t c)
+let print_st_typing #g #t #c (d:st_typing g t c)
   : T.Tac string 
-  = match d with
-    | T_Abs g x q b u body c tt body_typing ->
-      Printf.sprintf "(T_Abs ... %s)" (print_st_typing body_typing)
+  = "st typing is erased and cannot be printed"
+  // match d with
+  //   | T_Abs g x q b u body c tt body_typing ->
+  //     Printf.sprintf "(T_Abs ... %s)" (print_st_typing body_typing)
     
-    | T_STApp .. ->
-      "T_STApp"
+  //   | T_STApp .. ->
+  //     "T_STApp"
 
-    | T_STGhostApp .. ->
-      "T_STGhostApp"
+  //   | T_STGhostApp .. ->
+  //     "T_STGhostApp"
 
-    | T_Return .. ->
-      "T_Return"
+  //   | T_Return .. ->
+  //     "T_Return"
 
-    | T_Lift _ _ _ _ d _ ->
-      Printf.sprintf "(T_Lift %s)" (print_st_typing d)
+  //   | T_Lift _ _ _ _ d _ ->
+  //     Printf.sprintf "(T_Lift %s)" (print_st_typing d)
 
-    | T_Bind g e1 e2 c1 c2 b x c d1 _ d2 _ ->
-      Printf.sprintf "(T_Bind %s %s)" (print_st_typing d1) (print_st_typing d2)
+  //   | T_Bind g e1 e2 c1 c2 b x c d1 _ d2 _ ->
+  //     Printf.sprintf "(T_Bind %s %s)" (print_st_typing d1) (print_st_typing d2)
 
-    | T_BindFn _ _ _ _ _ _ _ d1 _ _ d2 _ ->
-      Printf.sprintf "(T_BindFn %s %s)" (print_st_typing d1) (print_st_typing d2)
+  //   | T_BindFn _ _ _ _ _ _ _ d1 _ _ d2 _ ->
+  //     Printf.sprintf "(T_BindFn %s %s)" (print_st_typing d1) (print_st_typing d2)
     
-    | T_If .. ->
-      "T_If"
+  //   | T_If .. ->
+  //     "T_If"
 
-    | T_Match .. ->
-      "T_Match"
+  //   | T_Match .. ->
+  //     "T_Match"
     
-    | T_Frame g e c frame _ body ->
-      Printf.sprintf "(T_Frame %s %s)" (Pulse.Syntax.Printer.term_to_string frame) (print_st_typing body)
+  //   | T_Frame g e c frame _ body ->
+  //     Printf.sprintf "(T_Frame %s %s)" (Pulse.Syntax.Printer.term_to_string frame) (print_st_typing body)
 
-    | T_Equiv g e c c' d eq ->
-      Printf.sprintf "(T_Equiv \n\t{%s}\n\t{%s}\n\t %s)"
-         (Pulse.Syntax.Printer.comp_to_string c)
-         (Pulse.Syntax.Printer.comp_to_string c')
-         (print_st_typing d)
+  //   | T_Equiv g e c c' d eq ->
+  //     Printf.sprintf "(T_Equiv \n\t{%s}\n\t{%s}\n\t %s)"
+  //        (Pulse.Syntax.Printer.comp_to_string c)
+  //        (Pulse.Syntax.Printer.comp_to_string c')
+  //        (print_st_typing d)
         
       
-    | T_Sub _ _ _ _ d _ -> 
-      Printf.sprintf "(T_Sub %s)" (print_st_typing d)
+  //   | T_Sub _ _ _ _ d _ -> 
+  //     Printf.sprintf "(T_Sub %s)" (print_st_typing d)
 
-    | T_IntroPure .. ->
-      "T_IntroPure"
+  //   | T_IntroPure .. ->
+  //     "T_IntroPure"
 
-    | T_ElimExists .. ->
-      "T_ElimExists"
+  //   | T_ElimExists .. ->
+  //     "T_ElimExists"
 
-    | T_IntroExists .. ->
-      "T_IntroExists"
+  //   | T_IntroExists .. ->
+  //     "T_IntroExists"
     
-    | T_While _ _ _ _ _ d1 d2 ->
-      Printf.sprintf "(T_While %s %s)" (print_st_typing d1) (print_st_typing d2)
+  //   | T_While _ _ _ _ _ d1 d2 ->
+  //     Printf.sprintf "(T_While %s %s)" (print_st_typing d1) (print_st_typing d2)
 
-    | T_WithLocal _ _ _ _ _ _ _ _ _ _ d ->
-      Printf.sprintf "(T_WithLocal %s)" (print_st_typing d)
+  //   | T_WithLocal _ _ _ _ _ _ _ _ _ _ d ->
+  //     Printf.sprintf "(T_WithLocal %s)" (print_st_typing d)
 
-    | T_WithLocalArray _ _ _ _ _ _ _ _ _ _ _ _ d ->
-      Printf.sprintf "(T_WithLocalArray %s)" (print_st_typing d)  
+  //   | T_WithLocalArray _ _ _ _ _ _ _ _ _ _ _ _ d ->
+  //     Printf.sprintf "(T_WithLocalArray %s)" (print_st_typing d)  
 
-    | T_Rewrite .. ->
-      "T_Rewrite"
+  //   | T_Rewrite .. ->
+  //     "T_Rewrite"
       
-    | T_Admit .. ->
-      "T_Admit"
+  //   | T_Admit .. ->
+  //     "T_Admit"
 
-    | T_Unreachable .. ->
-      "T_Unreachable"
+  //   | T_Unreachable .. ->
+  //     "T_Unreachable"
 
-    | T_WithInv _ _ _ _ _ _ _ d _ ->
-      Printf.sprintf "(T_WithInv %s)" (print_st_typing d)
+  //   | T_WithInv _ _ _ _ _ _ _ d _ ->
+  //     Printf.sprintf "(T_WithInv %s)" (print_st_typing d)
     
-    | T_Par _ _ _ _ _ _ _ _ d1 d2 ->
-      Printf.sprintf "(T_Par %s %s)" (print_st_typing d1) (print_st_typing d2)
+  //   | T_Par _ _ _ _ _ _ _ _ d1 d2 ->
+  //     Printf.sprintf "(T_Par %s %s)" (print_st_typing d1) (print_st_typing d2)
       
